updates

Veritas.Verifier.Correctness.fst
@@ -1,12 +1,15 @@
 module Veritas.Verifier.Correctness
 
 open FStar.Seq
+open Veritas.EAC
 open Veritas.Hash
 open Veritas.Interleave
 open Veritas.Key
 open Veritas.MultiSetHash
 open Veritas.Record
 open Veritas.SeqAux
+open Veritas.SeqMachine
+open Veritas.StateSeqMachine
 open Veritas.State
 open Veritas.Verifier
 
@@ -14,38 +17,38 @@ open Veritas.Verifier
 //Allow the solver to invert inductive definitions at most once (ifuel)
 #push-options "--max_fuel 1 --max_ifuel 1 --initial_fuel 1 --initial_ifuel 1"
 
-(* 
- * an indexed vlog attaches an nat index to a vlog 
+(*
+ * an indexed vlog attaches an nat index to a vlog
  * indicating the id of the verifier thread processing
- * the log 
+ * the log
  *)
 type tid_vlog = nat * vlog
 
 (* thread id of the indexed vlog *)
-let tid (il: tid_vlog) = fst il
+let tid (il: tid_vlog): nat = fst il
 
 (* vlog of an indexed vlog *)
-let vlog_of (il: tid_vlog) = snd il
+let vlog_of (il: tid_vlog): vlog = snd il
 
 (* length of the vlog portion *)
-let tv_length (tl: tid_vlog) = 
+let tv_length (tl: tid_vlog): nat =
   length (vlog_of tl)
 
 (* element at the i'th position of the vlog *)
-let tv_index (tl: tid_vlog) (i:nat{i < tv_length tl}) = 
+let tv_index (tl: tid_vlog) (i:nat{i < tv_length tl}): vlog_entry =
   index (vlog_of tl) i
 
 (* append an element at the end of the vlog *)
-let tv_append1 (tl: tid_vlog) (e: vlog_entry): Tot tid_vlog = 
+let tv_append1 (tl: tid_vlog) (e: vlog_entry): tid_vlog =
   (tid tl), (append1 (vlog_of tl) e)
 
-(* prefix of a tid_vlog: apply prefix on the 
+(* prefix of a tid_vlog: apply prefix on the
  * vlog component *)
-let tv_prefix (tl: tid_vlog) (i:nat{i <= tv_length tl}): Tot tid_vlog = 
+let tv_prefix (tl: tid_vlog) (i:nat{i <= tv_length tl}): tid_vlog =
   (tid tl), (prefix (vlog_of tl) i)
 
 (* does the log leave the verifier thread in a valid state *)
-let t_verifiable (il: tid_vlog) = 
+let t_verifiable (il: tid_vlog): bool =
   Valid? (t_verify (tid il) (vlog_of il))
 
 (* refinement types of valid verifier logs *)
@@ -54,7 +57,7 @@ type t_verifiable_log = il: tid_vlog {t_verifiable il}
 (* Full collection of verifier logs one per thread *)
 type g_vlog = seq vlog
 
-(* a slightly different view of verifier log obtained by 
+(* a slightly different view of verifier log obtained by
  * attaching a tid (index) to each thread verifier log *)
 let g_tid_vlog (gl: g_vlog) = attach_index gl
 
@@ -65,39 +68,39 @@ type g_verifiable (gl:g_vlog) = all t_verifiable (g_tid_vlog gl)
 type g_verifiable_log = l:g_vlog{g_verifiable l}
 
 (* view gl as a sequence of t_verifiable_logs *)
-let g_verifiable_refine (gl: g_verifiable_log): Tot (seq t_verifiable_log)
+let g_verifiable_refine (gl: g_verifiable_log): seq t_verifiable_log
   = seq_refine t_verifiable (g_tid_vlog gl)
 
 (* aggregate hadd over all verifier threads *)
-let g_hadd (gl: g_verifiable_log) = 
+let g_hadd (gl: g_verifiable_log): ms_hash_value =
   let th = fun (tl:t_verifiable_log) -> (thread_hadd (t_verify (fst tl) (snd tl))) in
-  let f = fun (tl:t_verifiable_log) (h:ms_hash_value) -> (ms_hashfn_agg (th tl) h) in     
+  let f = fun (tl:t_verifiable_log) (h:ms_hash_value) -> (ms_hashfn_agg (th tl) h) in
   reduce empty_hash_value f (g_verifiable_refine gl)
 
 (* aggregate hadd over all verifier threads *)
-let g_hevict (gl: g_verifiable_log) = 
+let g_hevict (gl: g_verifiable_log): ms_hash_value =
   let th = fun (tl:t_verifiable_log) -> (thread_hevict (t_verify (fst tl) (snd tl))) in
-  let f = fun (tl:t_verifiable_log) (h:ms_hash_value) -> (ms_hashfn_agg (th tl) h) in     
-  reduce empty_hash_value f (g_verifiable_refine gl)  
+  let f = fun (tl:t_verifiable_log) (h:ms_hash_value) -> (ms_hashfn_agg (th tl) h) in
+  reduce empty_hash_value f (g_verifiable_refine gl)
 
-(* 
- * a global log is hash verifiable if add and 
+(*
+ * a global log is hash verifiable if add and
  * evict hashes agree
  *)
-let g_hash_verifiable (lg: g_verifiable_log) = 
+let g_hash_verifiable (lg: g_verifiable_log): bool =
   g_hadd lg = g_hevict lg
 
 (* refinement type of hash verifiable log *)
-let g_hash_verifiable_log = 
+type g_hash_verifiable_log =
   lg:g_verifiable_log {g_hash_verifiable lg}
 
 let rec lemma_verifiable_implies_prefix_verifiable
   (tl:t_verifiable_log) (i:nat{i <= tv_length tl}):
   Lemma (requires (True))
         (ensures (t_verifiable (tv_prefix tl i)))
-        (decreases (tv_length tl)) 
+        (decreases (tv_length tl))
         [SMTPat (tv_prefix tl i)]
-        =    
+        =
   let n = tv_length tl in
   if n = 0 then ()
   else if i = n then ()
@@ -105,16 +108,16 @@ let rec lemma_verifiable_implies_prefix_verifiable
     lemma_verifiable_implies_prefix_verifiable (tv_prefix tl (n - 1)) i
 
 (* the clock of a verifier thread after processing a verifiable log *)
-let clock_after (tl:t_verifiable_log) = 
+let clock_after (tl:t_verifiable_log): timestamp =
   let vs = t_verify (tid tl) (vlog_of tl) in
   Valid?.clk vs
 
 (* the clock of a verifier is monotonic *)
 let rec lemma_clock_monotonic (tl:t_verifiable_log) (i:nat{i <= tv_length tl}):
   Lemma (requires(True))
-        (ensures (clock_after (tv_prefix tl i) `ts_leq` clock_after tl)) 
-  (decreases (tv_length tl))        
-        = 
+        (ensures (clock_after (tv_prefix tl i) `ts_leq` clock_after tl))
+  (decreases (tv_length tl))
+        =
   let n = tv_length tl in
   if n = 0 then ()
   else if i = n then ()
@@ -123,51 +126,120 @@ let rec lemma_clock_monotonic (tl:t_verifiable_log) (i:nat{i <= tv_length tl}):
     lemma_clock_monotonic tl' i
 
 (* We assign a time to every entry thread log *)
-let t_entry_time (tl: t_verifiable_log) (i:nat{i < tv_length tl}) =   
-  let tl' = tv_prefix tl (i+1) in  
+let t_entry_time (tl: t_verifiable_log) (i:nat{i < tv_length tl}): timestamp =
+  let tl' = tv_prefix tl (i+1) in
   clock_after tl'
 
 (* the clock of entry j <= clock of entry i if j occurs before i *)
 let lemma_time_monotonic_in_thread (tl: t_verifiable_log) (i:nat{i < tv_length tl}) (j:nat{j <= i}):
   Lemma (requires (True))
-        (ensures (t_entry_time tl j `ts_leq` t_entry_time tl i)) = 
+        (ensures (t_entry_time tl j `ts_leq` t_entry_time tl i)) =
   let tli = tv_prefix tl (i + 1) in
   lemma_clock_monotonic tli (j + 1)
 
 (* Time of an entry in global verifiable log *)
-let g_entry_time (gl: g_verifiable_log) (i: sseq_index gl) = admit()
+let g_entry_time (gl: g_verifiable_log) (si: sseq_index gl): timestamp =
+  let (i,j) = si in
+  let tl = index (g_tid_vlog gl) i in
+  t_entry_time tl j
 
-(* define time sequence obtained by ordering all log entries across all threads 
+(* define time sequence obtained by ordering all log entries across all threads
  * by their assigned time as defined above *)
-let time_seq_ctor (gl: g_verifiable_log): 
+let time_seq_ctor (gl: g_verifiable_log):
   Tot (interleave_ctor gl) =
   admit()
 
-let time_seq (gl: g_verifiable_log) = interleaved_seq gl (time_seq_ctor gl)
+let time_seq (gl: g_verifiable_log)
+  = interleaved_seq gl (time_seq_ctor gl)
 
 (* map every entry of the time sequence to its source entry in the thread logs *)
-let time_seq_source (gl: g_verifiable_log) (i: seq_index (time_seq gl)) =
+let time_seq_source (gl: g_verifiable_log) (i: seq_index (time_seq gl)): sseq_index gl =
   interleave_map (time_seq gl) gl (interleaving_prf gl (time_seq_ctor gl)) i
 
 (* if i <= j are two indexes in the time_seq, then the time of entry i <= time of entry j*)
-let lemma_time_seq_correct (gl: g_verifiable_log) 
+let lemma_time_seq_correct (gl: g_verifiable_log)
                            (i: seq_index (time_seq gl))
                            (j: seq_index (time_seq gl){j >= i}):
-  Lemma (g_entry_time gl (time_seq_source gl i) <= g_entry_time gl (time_seq_source gl j)) = admit()
+  Lemma (g_entry_time gl (time_seq_source gl i) `ts_leq` g_entry_time gl (time_seq_source gl j))
+  = admit()
 
-
-
-(*
 (* state ops of all vlogs of all verifier threads *)
-let to_state_op_gvlog (gl: g_vlog) = 
+let to_state_op_gvlog (gl: g_vlog) =
   map to_state_op_vlog gl
 
 (* generalized single- and multi-set hash collision *)
-type hash_collision_gen = 
-  | SingleHashCollision: hc: hash_collision -> hash_collision_gen 
+type hash_collision_gen =
+  | SingleHashCollision: hc: hash_collision -> hash_collision_gen
   | MultiHashCollision: hc: ms_hash_collision -> hash_collision_gen
 
+
+let time_seq_ext (gl: g_verifiable_log):
+  (le:vlog_ext{to_vlog le = time_seq gl})
+  = admit()
+
+let lemma_time_seq_not_eac_implies_hash_collision
+  (gl: g_hash_verifiable_log { ~ (eac (time_seq_ext gl)) }): hash_collision_gen = admit()
+
+let lemma_time_seq_rw_consistent
+  (gl: g_hash_verifiable_log { ~ (rw_consistent (to_state_op_vlog (time_seq gl)))}): hash_collision_gen =
+
+  (* time sequence log *)
+  let tmsle = time_seq_ext gl in
+  let tmsl = time_seq gl in
+
+  (* sequence of state ops in time sequence *)
+  let tm_ops = to_state_op_vlog tmsl in
+  assert(~ (rw_consistent tm_ops));
+
+  (* is time seq log evict add consistent? *)
+  let is_eac = valid_all_comp eac_sm tmsle in
+
+  (* if tmsle is evict add consistent then tm_ops is rw_consistent, a contradiction *)
+  if is_eac then (
+     lemma_eac_implies_rw_consistent tmsle;
+     assert(rw_consistent tm_ops);
+
+     (* any return value *)
+     SingleHashCollision (Collision (DVal Null) (DVal Null))
+  )
+  else
+    lemma_time_seq_not_eac_implies_hash_collision gl
+
+let lemma_vlog_interleave_implies_state_ops_interleave (l: vlog) (gl: g_vlog{interleave l gl}):
+  Lemma (interleave (to_state_op_vlog l) (to_state_op_gvlog gl)) = admit()
+
 (* final verifier correctness theorem *)
-let lemma_verifier_correct (lg: g_hash_verifiable_log { ~ (seq_consistent (to_state_op_gvlog lg))}):
-  Tot hash_collision_gen = admit()
-  *)
+let lemma_verifier_correct (gl: g_hash_verifiable_log { ~ (seq_consistent (to_state_op_gvlog gl))}):
+  hash_collision_gen =
+
+  (* sequences of per-thread put/get operations *)
+  let g_ops = to_state_op_gvlog gl in
+
+  (* sequence ordered by time of each log entry *)
+  let tmsl = time_seq gl in
+  assert(interleave tmsl gl);
+
+  (* sequence of state ops induced by tmsl *)
+  let tm_ops = to_state_op_vlog tmsl in
+
+  lemma_vlog_interleave_implies_state_ops_interleave tmsl gl;
+  assert(interleave tm_ops g_ops);
+
+  (* if tm_ops is read-write consistent then we have a contradiction *)
+  let is_rw_consistent = valid_all_comp ssm tm_ops in
+
+  if is_rw_consistent then (
+
+    assert(valid_all ssm tm_ops);
+    lemma_state_sm_equiv_rw_consistent tm_ops;
+    assert(rw_consistent tm_ops);
+
+    (* a contradiction *)
+    assert(seq_consistent g_ops);
+
+    (* any return value *)
+    SingleHashCollision (Collision (DVal Null) (DVal Null))
+  )
+  else
+    (* otherwise we can produce a collision *)
+    lemma_time_seq_rw_consistent gl
